Instances/ISAs/VexSummary.lean
@@ -15,6 +15,7 @@ inductive SymExpr (Reg : Type) where
   | sext8to32 : SymExpr Reg → SymExpr Reg
   | sext32to64 : SymExpr Reg → SymExpr Reg
   | sub32 : SymExpr Reg → SymExpr Reg → SymExpr Reg
+  | shl32 : SymExpr Reg → SymExpr Reg → SymExpr Reg
   | add64 : SymExpr Reg → SymExpr Reg → SymExpr Reg
   | sub64 : SymExpr Reg → SymExpr Reg → SymExpr Reg
   | xor64 : SymExpr Reg → SymExpr Reg → SymExpr Reg
@@ -135,6 +136,7 @@ mutual
   | .sext8to32 expr => signExtend8to32 (evalSymExpr state expr)
   | .sext32to64 expr => signExtend32to64 (evalSymExpr state expr)
   | .sub32 lhs rhs => mask32 (evalSymExpr state lhs - evalSymExpr state rhs)
+  | .shl32 lhs rhs => shiftLeft32 (evalSymExpr state lhs) (evalSymExpr state rhs)
   | .add64 lhs rhs => evalSymExpr state lhs + evalSymExpr state rhs
   | .sub64 lhs rhs => evalSymExpr state lhs - evalSymExpr state rhs
   | .xor64 lhs rhs => evalSymExpr state lhs ^^^ evalSymExpr state rhs
@@ -175,6 +177,7 @@ def substSymExpr {Reg : Type} [DecidableEq Reg] [Fintype Reg]
   | .sext8to32 expr => .sext8to32 (substSymExpr sub expr)
   | .sext32to64 expr => .sext32to64 (substSymExpr sub expr)
   | .sub32 lhs rhs => .sub32 (substSymExpr sub lhs) (substSymExpr sub rhs)
+  | .shl32 lhs rhs => .shl32 (substSymExpr sub lhs) (substSymExpr sub rhs)
   | .add64 lhs rhs => .add64 (substSymExpr sub lhs) (substSymExpr sub rhs)
   | .sub64 lhs rhs => .sub64 (substSymExpr sub lhs) (substSymExpr sub rhs)
   | .xor64 lhs rhs => .xor64 (substSymExpr sub lhs) (substSymExpr sub rhs)
@@ -263,6 +266,8 @@ theorem substSymExpr_id {Reg : Type} [DecidableEq Reg] [Fintype Reg] (expr : Sym
   | sext32to64 expr => simp [substSymExpr, substSymExpr_id]
   | sub32 lhs rhs =>
       simp [substSymExpr, substSymExpr_id]
+  | shl32 lhs rhs =>
+      simp [substSymExpr, substSymExpr_id]
   | add64 lhs rhs =>
       simp [substSymExpr, substSymExpr_id]
   | sub64 lhs rhs =>
@@ -300,6 +305,8 @@ theorem substSymExpr_compose {Reg : Type} [DecidableEq Reg] [Fintype Reg]
   | sext8to32 expr => simp [substSymExpr, substSymExpr_compose]
   | sext32to64 expr => simp [substSymExpr, substSymExpr_compose]
   | sub32 lhs rhs =>
+      simp [substSymExpr, substSymExpr_compose]
+  | shl32 lhs rhs =>
       simp [substSymExpr, substSymExpr_compose]
   | add64 lhs rhs =>
       simp [substSymExpr, substSymExpr_compose]
@@ -339,6 +346,8 @@ theorem evalSymExpr_subst {Reg : Type} [DecidableEq Reg] [Fintype Reg]
   | sext8to32 expr => simp [substSymExpr, evalSymExpr_subst]
   | sext32to64 expr => simp [substSymExpr, evalSymExpr_subst]
   | sub32 lhs rhs =>
+      simp [substSymExpr, evalSymExpr_subst]
+  | shl32 lhs rhs =>
       simp [substSymExpr, evalSymExpr_subst]
   | add64 lhs rhs =>
       simp [substSymExpr, evalSymExpr_subst]
